examples/hwmcc_checker/translation/aig_fmapsProgScript.sml
@@ -1,9 +1,9 @@
 (*
-  Setting up translator for the fmap instances that are used in aig_to_cnf.
+  Setting up translator for the fmap instances that are used in xaig_to_cnf.
 *)
 Theory aig_fmapsProg
 Ancestors
-  aig_cert_encodeProg aig_to_cnf
+  aig_cert_encodeProg xaig_to_cnf
 Libs
   preamble ml_translatorLib MapProgLib
 
@@ -11,19 +11,21 @@ val _ = translation_extends "aig_cert_encodeProg";
 
 (*----------------------------------------------------------------------*
    specific types to target
+
+   ty1-ty3 are the input and latch types of the encoded conditions; ty4-ty9
+   are their gate name types, which is what the renaming in xrename_to_cnf
+   is keyed by.  Everything after that renaming is at ty1.
  *----------------------------------------------------------------------*)
 
 Type ty1[local] = “:num”;
 Type ty2[local] = “:num + num”;
-Type ty3[local] = “:num iext”;
-Type ty4[local] = “:(num + num) iext”;
-Type ty5[local] = “:(num iext + num iext) iext”;
-Type ty6[local] = “:((num + num) iext + (num + num) iext) iext”;
-Type ty7[local] = “:(ty6 + ty4) iext”
-Type ty8[local] = “:(ty5 + ty3) iext”
-Type ty9[local] = “:(((ty8 + ty3) iext) + ty3) iext”
-Type ty10[local] = “:(ty8 + ty4) iext”
-Type ty11[local] = “:(num + num) + num”
+Type ty3[local] = “:ty2 + num”;
+Type ty4[local] = “:num ext”;
+Type ty5[local] = “:ty2 ext”;
+Type ty6[local] = “:(ty2 + ty2) ext”;
+Type ty7[local] = “:((ty2 + ty2) + ty2) ext”;
+Type ty8[local] = “:ty3 ext”;
+Type ty9[local] = “:(ty3 + ty2) ext”;
 
 (*----------------------------------------------------------------------*
    ty1
@@ -59,40 +61,46 @@ QED
    ty3
  *----------------------------------------------------------------------*)
 
+Definition ty3_cmp_def:
+  ty3_cmp = sum_cmp num_sum_num_cmp num_cmp
+End
+
+Theorem ty3_cmp_eq[local] =
+  ty3_cmp_def |> SRULE [sum_cmp_def, num_sum_num_cmp_eq, num_cmp_thm, FUN_EQ_THM];
+
+val r = translate ty3_cmp_eq;
+
+Theorem TotOrd_ty3:
+  TotOrd (ty3_cmp : ty3 -> ty3 -> ordering)
+Proof
+  rewrite_tac [ty3_cmp_def]
+  \\ irule TotOrd_sum \\ simp [TotOrd_ty2, TotOrd_ty1]
+QED
+
+(*----------------------------------------------------------------------*
+   the ext wrapper
+ *----------------------------------------------------------------------*)
+
 Definition ext_cmp_def:
   ext_cmp cmp (x1: 'a ext) (x2: 'a ext) =
     case x1 of
     | Orig n1 =>
         (case x2 of
          | Orig n2 => cmp n1 n2
-         | Ext _ => LESS)
+         | _ => LESS)
     | Ext n1 =>
         (case x2 of
          | Orig _ => GREATER
-         | Ext n2 => mlstring$compare n1 n2)
-End
-
-Definition iext_cmp_def:
-  iext_cmp cmp (x1: 'a iext) (x2: 'a iext) =
-    case x1 of
-    | Named n1 =>
-        (case x2 of
-         | Named n2 => ext_cmp cmp n1 n2
+         | Ext n2 => mlstring$compare n1 n2
          | Anon _ => LESS)
     | Anon n1 =>
         (case x2 of
-         | Named _ => GREATER
-         | Anon n2 => num_cmp n1 n2)
+         | Anon n2 => num_cmp n1 n2
+         | _ => GREATER)
 End
 
 Theorem ext_forall:
-  (∀x. P x) ⇔ (∀y. P (Orig y)) ∧ (∀y. P (Ext y))
-Proof
-  eq_tac \\ rw [] \\ simp [] \\ Cases_on ‘x’ \\ fs []
-QED
-
-Theorem iext_forall:
-  (∀x. P x) ⇔ (∀y. P (Named y)) ∧ (∀y. P (Anon y))
+  (∀x. P x) ⇔ (∀y. P (Orig y)) ∧ (∀y. P (Ext y)) ∧ (∀y. P (Anon y))
 Proof
   eq_tac \\ rw [] \\ simp [] \\ Cases_on ‘x’ \\ fs []
 QED
@@ -100,91 +108,56 @@ QED
 Theorem TotOrd_ext:
   TotOrd c1 ⇒ TotOrd (ext_cmp c1)
 Proof
-  mp_tac mlstringTheory.TotOrd_compare
+  strip_tac
+  \\ mp_tac mlstringTheory.TotOrd_compare
+  \\ mp_tac TotOrd_ty1
   \\ fs [totoTheory.TotOrd, ext_cmp_def, AllCaseEqs(), ext_forall]
   \\ simp [SF DNF_ss, PULL_EXISTS] \\ rw [] \\ res_tac
 QED
 
-Theorem TotOrd_iext:
-  TotOrd c1 ⇒ TotOrd (iext_cmp c1)
-Proof
-  strip_tac \\ dxrule TotOrd_ext
-  \\ mp_tac TotOrd_ty1
-  \\ fs [totoTheory.TotOrd, iext_cmp_def, AllCaseEqs(), iext_forall]
-  \\ simp [SF DNF_ss, PULL_EXISTS] \\ rw [] \\ res_tac
-QED
-
-Definition num_iext_cmp_def:
-  num_iext_cmp = iext_cmp num_cmp
-End
-
-Theorem num_iext_cmp_eq[local] =
-  num_iext_cmp_def |> SRULE [iext_cmp_def, num_cmp_thm, FUN_EQ_THM, ext_cmp_def];
-
-val r = translate num_iext_cmp_eq;
-
-Theorem TotOrd_ty3:
-  TotOrd (num_iext_cmp : ty3 -> ty3 -> ordering)
-Proof
-  rewrite_tac [num_iext_cmp_def]
-  \\ irule TotOrd_iext \\ simp [TotOrd_ty1]
-QED
-
 (*----------------------------------------------------------------------*
-   ty4
+   ty4 - ty9
  *----------------------------------------------------------------------*)
 
 Definition ty4_cmp_def:
-  ty4_cmp = iext_cmp num_sum_num_cmp
+  ty4_cmp = ext_cmp num_cmp
 End
 
 Theorem ty4_cmp_eq[local] =
-  ty4_cmp_def
-  |> SRULE [iext_cmp_def, num_sum_num_cmp_eq, FUN_EQ_THM, ext_cmp_def, num_cmp_thm];
+  ty4_cmp_def |> SRULE [ext_cmp_def, num_cmp_thm, FUN_EQ_THM];
 
 val r = translate ty4_cmp_eq;
 
 Theorem TotOrd_ty4:
   TotOrd (ty4_cmp : ty4 -> ty4 -> ordering)
 Proof
-  rewrite_tac [ty4_cmp_def]
-  \\ irule TotOrd_iext \\ simp [TotOrd_ty2]
+  rewrite_tac [ty4_cmp_def] \\ irule TotOrd_ext \\ simp [TotOrd_ty1]
 QED
 
-(*----------------------------------------------------------------------*
-   ty5
- *----------------------------------------------------------------------*)
-
 Definition ty5_cmp_def:
-  ty5_cmp = iext_cmp (sum_cmp num_iext_cmp num_iext_cmp)
+  ty5_cmp = ext_cmp num_sum_num_cmp
 End
 
 Theorem ty5_cmp_eq[local] =
   ty5_cmp_def
-  |> SRULE [iext_cmp_def, FUN_EQ_THM, ext_cmp_def, num_cmp_thm, sum_cmp_def];
+  |> SRULE [ext_cmp_def, num_sum_num_cmp_eq, num_cmp_thm, FUN_EQ_THM];
 
 val r = translate ty5_cmp_eq;
 
 Theorem TotOrd_ty5:
   TotOrd (ty5_cmp : ty5 -> ty5 -> ordering)
 Proof
-  rewrite_tac [ty5_cmp_def]
-  \\ irule TotOrd_iext
-  \\ irule TotOrd_sum
-  \\ simp [TotOrd_ty3]
+  rewrite_tac [ty5_cmp_def] \\ irule TotOrd_ext \\ simp [TotOrd_ty2]
 QED
 
-(*----------------------------------------------------------------------*
-   ty6
- *----------------------------------------------------------------------*)
-
 Definition ty6_cmp_def:
-  ty6_cmp = iext_cmp (sum_cmp ty4_cmp ty4_cmp)
+  ty6_cmp = ext_cmp (sum_cmp num_sum_num_cmp num_sum_num_cmp)
 End
 
 Theorem ty6_cmp_eq[local] =
   ty6_cmp_def
-  |> SRULE [iext_cmp_def, FUN_EQ_THM, ext_cmp_def, num_cmp_thm, sum_cmp_def];
+  |> SRULE [ext_cmp_def, sum_cmp_def, num_sum_num_cmp_eq, num_cmp_thm,
+            FUN_EQ_THM];
 
 val r = translate ty6_cmp_eq;
 
@@ -192,22 +165,18 @@ Theorem TotOrd_ty6:
   TotOrd (ty6_cmp : ty6 -> ty6 -> ordering)
 Proof
   rewrite_tac [ty6_cmp_def]
-  \\ irule TotOrd_iext
-  \\ irule TotOrd_sum
-  \\ simp [TotOrd_ty4]
+  \\ irule TotOrd_ext \\ irule TotOrd_sum \\ simp [TotOrd_ty2]
 QED
 
-(*----------------------------------------------------------------------*
-   ty7
- *----------------------------------------------------------------------*)
-
 Definition ty7_cmp_def:
-  ty7_cmp = iext_cmp (sum_cmp ty6_cmp ty4_cmp)
+  ty7_cmp =
+    ext_cmp (sum_cmp (sum_cmp num_sum_num_cmp num_sum_num_cmp) num_sum_num_cmp)
 End
 
 Theorem ty7_cmp_eq[local] =
   ty7_cmp_def
-  |> SRULE [iext_cmp_def, FUN_EQ_THM, ext_cmp_def, num_cmp_thm, sum_cmp_def];
+  |> SRULE [ext_cmp_def, sum_cmp_def, num_sum_num_cmp_eq, num_cmp_thm,
+            FUN_EQ_THM];
 
 val r = translate ty7_cmp_eq;
 
@@ -215,45 +184,34 @@ Theorem TotOrd_ty7:
   TotOrd (ty7_cmp : ty7 -> ty7 -> ordering)
 Proof
   rewrite_tac [ty7_cmp_def]
-  \\ irule TotOrd_iext
-  \\ irule TotOrd_sum
-  \\ simp [TotOrd_ty6, TotOrd_ty4]
+  \\ irule TotOrd_ext \\ irule TotOrd_sum
+  \\ irule_at (Pos hd) TotOrd_sum
+  \\ simp [TotOrd_ty2]
 QED
 
-(*----------------------------------------------------------------------*
-   ty8
- *----------------------------------------------------------------------*)
-
 Definition ty8_cmp_def:
-  ty8_cmp = iext_cmp (sum_cmp ty5_cmp num_iext_cmp)
+  ty8_cmp = ext_cmp ty3_cmp
 End
 
 Theorem ty8_cmp_eq[local] =
-  ty8_cmp_def
-  |> SRULE [iext_cmp_def, FUN_EQ_THM, ext_cmp_def, num_cmp_thm, sum_cmp_def];
+  ty8_cmp_def |> SRULE [ext_cmp_def, ty3_cmp_eq, num_cmp_thm, FUN_EQ_THM];
 
 val r = translate ty8_cmp_eq;
 
 Theorem TotOrd_ty8:
   TotOrd (ty8_cmp : ty8 -> ty8 -> ordering)
 Proof
-  rewrite_tac [ty8_cmp_def]
-  \\ irule TotOrd_iext
-  \\ irule TotOrd_sum
-  \\ simp [TotOrd_ty5, TotOrd_ty3]
+  rewrite_tac [ty8_cmp_def] \\ irule TotOrd_ext \\ simp [TotOrd_ty3]
 QED
 
-(*----------------------------------------------------------------------*
-   ty9
- *----------------------------------------------------------------------*)
-
 Definition ty9_cmp_def:
-  ty9_cmp = iext_cmp (sum_cmp (iext_cmp (sum_cmp ty8_cmp num_iext_cmp)) num_iext_cmp)
+  ty9_cmp = ext_cmp (sum_cmp ty3_cmp num_sum_num_cmp)
 End
 
 Theorem ty9_cmp_eq[local] =
   ty9_cmp_def
-  |> SRULE [iext_cmp_def, FUN_EQ_THM, ext_cmp_def, num_cmp_thm, sum_cmp_def];
+  |> SRULE [ext_cmp_def, sum_cmp_def, ty3_cmp_eq, num_sum_num_cmp_eq,
+            num_cmp_thm, FUN_EQ_THM];
 
 val r = translate ty9_cmp_eq;
 
@@ -261,56 +219,7 @@ Theorem TotOrd_ty9:
   TotOrd (ty9_cmp : ty9 -> ty9 -> ordering)
 Proof
   rewrite_tac [ty9_cmp_def]
-  \\ irule TotOrd_iext
-  \\ irule TotOrd_sum
-  \\ irule_at (Pos hd) TotOrd_iext
-  \\ irule_at (Pos hd) TotOrd_sum
-  \\ simp [TotOrd_ty8, TotOrd_ty3]
-QED
-
-(*----------------------------------------------------------------------*
-   ty10
- *----------------------------------------------------------------------*)
-
-Definition ty10_cmp_def:
-  ty10_cmp = iext_cmp (sum_cmp ty8_cmp ty4_cmp)
-End
-
-Theorem ty10_cmp_eq[local] =
-  ty10_cmp_def
-  |> SRULE [iext_cmp_def, FUN_EQ_THM, ext_cmp_def, num_cmp_thm, sum_cmp_def];
-
-val r = translate ty10_cmp_eq;
-
-Theorem TotOrd_ty10:
-  TotOrd (ty10_cmp : ty10 -> ty10 -> ordering)
-Proof
-  rewrite_tac [ty10_cmp_def]
-  \\ irule TotOrd_iext
-  \\ irule TotOrd_sum
-  \\ simp [TotOrd_ty8, TotOrd_ty4]
-QED
-
-(*----------------------------------------------------------------------*
-   ty11
- *----------------------------------------------------------------------*)
-
-Definition ty11_cmp_def:
-  ty11_cmp = sum_cmp num_sum_num_cmp num_cmp
-End
-
-Theorem ty11_cmp_eq[local] =
-  ty11_cmp_def
-  |> SRULE [sum_cmp_def, num_sum_num_cmp_eq, num_cmp_thm, FUN_EQ_THM];
-
-val r = translate ty11_cmp_eq;
-
-Theorem TotOrd_ty11:
-  TotOrd (ty11_cmp : ty11 -> ty11 -> ordering)
-Proof
-  rewrite_tac [ty11_cmp_def]
-  \\ irule TotOrd_sum
-  \\ simp [TotOrd_ty2, TotOrd_ty1]
+  \\ irule TotOrd_ext \\ irule TotOrd_sum \\ simp [TotOrd_ty3, TotOrd_ty2]
 QED
 
 (*----------------------------------------------------------------------*
@@ -326,5 +235,3 @@ val _ = add_fmap_for_cmp TotOrd_ty6;
 val _ = add_fmap_for_cmp TotOrd_ty7;
 val _ = add_fmap_for_cmp TotOrd_ty8;
 val _ = add_fmap_for_cmp TotOrd_ty9;
-val _ = add_fmap_for_cmp TotOrd_ty10;
-val _ = add_fmap_for_cmp TotOrd_ty11;
