examples/hwmcc_checker/translation/aigProgScript.sml
@@ -1,9 +1,9 @@
 (*
-  Translates aig.
+  Translates aig and xaig.
 *)
 Theory aigProg
 Ancestors
-  aig basisProg
+  aig xaig basisProg
 Libs
   preamble ml_translatorLib
 
@@ -11,11 +11,19 @@ val _ = translation_extends "basisProg";
 
 val r = register_type “:('i, 'l) bvar”;
 val r = register_type “:('a, 'i, 'l) var”;
+val r = register_type “:('a, 'i, 'l) gty”;
 
 val r = translate aigTheory.not_def;
 
-val r = translate aigTheory.bvar_latches_def;
-val r = translate aigTheory.var_latches_def;
-val r = translate aigTheory.lit_latches_def;
-val r = translate aigTheory.and_latches_def;
-val r = translate aigTheory.aig_latches_def;
+val r = translate aigTheory.bvar_map_def;
+val r = translate aigTheory.var_map_base_def;
+val r = translate aigTheory.lit_map_base_def;
+val r = translate aigTheory.live_map_base_def;
+val r = translate aigTheory.qleft_live_def;
+
+val r = translate xaigTheory.get_lits_def;
+val r = translate xaigTheory.gty_map_base_def;
+val r = translate xaigTheory.gate_map_base_def;
+val r = translate xaigTheory.xaig_map_base_def;
+val r = translate xaigTheory.qxleft_def;
+val r = translate xaigTheory.aig_to_xaig_def;
