examples/hwmcc_checker/translation/aig_cert_encodeProgScript.sml
@@ -1,114 +1,109 @@
 (*
-  Translates aig_cert_encode.
+  Translates xaig_cert_encode.
 *)
 Theory aig_cert_encodeProg
 Ancestors
   ml_translator (* for MEMBER_INTRO *)
-  aig_cert_encode aig_parseProg
+  xaig_cert xaig_cert_encode aig_parseProg
 Libs
   preamble ml_translatorLib
 
 val _ = translation_extends "aig_parseProg";
 
 val r = register_type “:'a ext”;
-val r = register_type “:'a iext”;
 
-val r = translate aig_cert_encodeTheory.left_name_var_def;
-val r = translate aig_cert_encodeTheory.left_name_lit_def;
-val r = translate aig_cert_encodeTheory.left_name_and_def;
-val r = translate aig_cert_encodeTheory.right_name_var_def;
-val r = translate aig_cert_encodeTheory.right_name_lit_def;
-val r = translate aig_cert_encodeTheory.right_name_and_def;
-val r = translate aig_cert_encodeTheory.merge_aigs_def;
+val r = translate xaig_certTheory.bvar_latches_def;
+val r = translate xaig_certTheory.var_latches_def;
+val r = translate xaig_certTheory.lit_latches_def;
+val r = translate xaig_certTheory.gty_latches_def;
+val r = translate xaig_certTheory.gate_latches_def;
+val r = translate xaig_certTheory.xaig_latches_def;
 
-val r = translate aig_cert_encodeTheory.left_bvar_def;
-val r = translate aig_cert_encodeTheory.left_var_def;
-val r = translate aig_cert_encodeTheory.left_lit_def;
-val r = translate aig_cert_encodeTheory.left_and_def;
-val r = translate aig_cert_encodeTheory.right_bvar_def;
-val r = translate aig_cert_encodeTheory.right_var_def;
-val r = translate aig_cert_encodeTheory.right_lit_def;
-val r = translate aig_cert_encodeTheory.right_and_def;
-val r = translate aig_cert_encodeTheory.pair_aigs_def;
+val r = translate xaig_cert_encodeTheory.left_name_var_def;
+val r = translate xaig_cert_encodeTheory.left_name_lit_def;
+val r = translate xaig_cert_encodeTheory.left_name_gty_def;
+val r = translate xaig_cert_encodeTheory.left_name_gate_def;
+val r = translate xaig_cert_encodeTheory.right_name_var_def;
+val r = translate xaig_cert_encodeTheory.right_name_lit_def;
+val r = translate xaig_cert_encodeTheory.right_name_gty_def;
+val r = translate xaig_cert_encodeTheory.right_name_gate_def;
+val r = translate xaig_cert_encodeTheory.merge_xaigs_def;
 
-val r = translate aig_cert_encodeTheory.iext_var_def;
-val r = translate aig_cert_encodeTheory.iext_lit_def;
-val r = translate aig_cert_encodeTheory.iext_and_def;
-val r = translate aig_cert_encodeTheory.iext_aig_def;
+val r = translate xaig_cert_encodeTheory.left_bvar_def;
+val r = translate xaig_cert_encodeTheory.left_var_def;
+val r = translate xaig_cert_encodeTheory.left_lit_def;
+val r = translate xaig_cert_encodeTheory.left_gty_def;
+val r = translate xaig_cert_encodeTheory.left_gate_def;
+val r = translate xaig_cert_encodeTheory.right_bvar_def;
+val r = translate xaig_cert_encodeTheory.right_var_def;
+val r = translate xaig_cert_encodeTheory.right_lit_def;
+val r = translate xaig_cert_encodeTheory.right_gty_def;
+val r = translate xaig_cert_encodeTheory.right_gate_def;
+val r = translate xaig_cert_encodeTheory.pair_xaigs_def;
 
-val r = translate aig_cert_encodeTheory.iname_def;
+val r = translate xaig_cert_encodeTheory.qinterv_lit_def;
+val r = translate xaig_cert_encodeTheory.qinterv_gty_def;
+val r = translate xaig_cert_encodeTheory.qinterv_gate_def;
+val r = translate xaig_cert_encodeTheory.qinterv_live_def;
+val r = translate xaig_cert_encodeTheory.qinterv_def;
 
+val r = translate xaig_cert_encodeTheory.qinterv_l_r_def;
+val r = translate xaig_cert_encodeTheory.qinterv_live_l_r_def;
+val r = translate xaig_cert_encodeTheory.qinterv_live_r_l_def;
+val r = translate xaig_cert_encodeTheory.qinterv_live_ll_r_def;
+val r = translate xaig_cert_encodeTheory.qinterv_live_ll_lr_def;
+val r = translate xaig_cert_encodeTheory.qinterv_live_lr_r_def;
+val r = translate xaig_cert_encodeTheory.qinterv_r_l_def;
+val r = translate xaig_cert_encodeTheory.qinterv_ll_r_def;
+val r = translate xaig_cert_encodeTheory.qinterv_ll_lr_def;
+val r = translate xaig_cert_encodeTheory.qinterv_lr_r_def;
+
+val r = translate xaig_cert_encodeTheory.ext_var_def;
+val r = translate xaig_cert_encodeTheory.ext_lit_def;
+val r = translate xaig_cert_encodeTheory.ext_gty_def;
+val r = translate xaig_cert_encodeTheory.ext_gate_def;
+val r = translate xaig_cert_encodeTheory.ext_xaig_def;
+
+val r = translate xaig_cert_encodeTheory.iname_def;
 val r = translate rich_listTheory.MAX_LIST_def;
-val r = translate aig_cert_encodeTheory.maxn_def;
+val r = translate xaig_cert_encodeTheory.maxn_def;
 
-val r = translate aig_cert_encodeTheory.encode_imply_def;
-val r = translate aig_cert_encodeTheory.encode_equiv_aux_def;
-val r = translate aig_cert_encodeTheory.encode_equiv_def;
-val r = translate aig_cert_encodeTheory.latch_reset_pairs_def;
-val r = translate aig_cert_encodeTheory.encode_is_reset_def;
-val r = translate aig_cert_encodeTheory.encode_lits_hold_def;
+val r = translate xaig_cert_encodeTheory.encode_imply_def;
 
-val r = translate aig_cert_encodeTheory.left_reset_def;
-val r = translate aig_cert_encodeTheory.right_reset_def;
-val r = translate aig_cert_encodeTheory.iext_reset_def;
-val r = translate aig_cert_encodeTheory.ileft_reset_def;
-val r = translate aig_cert_encodeTheory.iright_reset_def;
-val r = translate aig_cert_encodeTheory.ileft_name_lits_def;
-val r = translate aig_cert_encodeTheory.iright_name_lits_def;
-val r = translate aig_cert_encodeTheory.imerge_aigs_def;
+val r = translate xaig_cert_encodeTheory.xori_def;
+val r = translate xaig_cert_encodeTheory.encode_pointwise_equal_def;
+val r = translate xaig_cert_encodeTheory.impi_def;
+val r = translate xaig_cert_encodeTheory.encode_pointwise_imply_def;
 
-val r = translate aig_cert_encodeTheory.encode_is_next_with_def;
-val r = translate aig_cert_encodeTheory.encode_is_next_def;
+val r = translate xaig_cert_encodeTheory.latch_reset_pairs_def;
+val r = translate xaig_cert_encodeTheory.encode_xis_reset_def;
+val r = translate xaig_cert_encodeTheory.encode_xlits_hold_def;
 
-val r = translate (miscTheory.list_inter_def |> SRULE [MEMBER_INTRO]);
+val r = translate xaig_cert_encodeTheory.ext_reset_def;
+val r = translate xaig_cert_encodeTheory.left_reset_def;
+val r = translate xaig_cert_encodeTheory.right_reset_def;
 
-val r = translate aig_cert_encodeTheory.bvar_map_def;
-val r = translate aig_cert_encodeTheory.var_map_base_def;
-val r = translate aig_cert_encodeTheory.lit_map_base_def;
-val r = translate aig_cert_encodeTheory.live_map_base_def;
-val r = translate aig_cert_encodeTheory.and_map_base_def;
-val r = translate aig_cert_encodeTheory.aig_map_base_def;
+val r = translate xaig_cert_encodeTheory.encode_xis_next_def;
 
-val r = translate aig_cert_encodeTheory.qleft_def;
-val r = translate aig_cert_encodeTheory.qleft_live_def;
+val r = translate xaig_cert_encodeTheory.encode_signal_imply_def;
+val r = translate xaig_cert_encodeTheory.ori_def;
+val r = translate xaig_cert_encodeTheory.encode_lives_hold_def;
 
-val r = translate aig_cert_encodeTheory.qinterv_lit_def;
-val r = translate aig_cert_encodeTheory.qinterv_and_def;
-val r = translate aig_cert_encodeTheory.qinterv_def;
-val r = translate aig_cert_encodeTheory.qinterv_l_r_def;
-val r = translate aig_cert_encodeTheory.qinterv_r_l_def;
-val r = translate aig_cert_encodeTheory.qinterv_lr_r_def;
-val r = translate aig_cert_encodeTheory.qinterv_ll_r_def;
-val r = translate aig_cert_encodeTheory.qinterv_ll_lr_def;
+val r = translate xaig_cert_encodeTheory.encode_reset_cond_def;
+val r = translate xaig_cert_encodeTheory.encode_transition_cond_def;
+val r = translate xaig_cert_encodeTheory.encode_safety_cond_def;
+val r = translate xaig_cert_encodeTheory.encode_base_cond_def;
+val r = translate xaig_cert_encodeTheory.encode_induction_cond_def;
 
-val r = translate aig_cert_encodeTheory.qinterv_live_def;
-val r = translate aig_cert_encodeTheory.qinterv_live_l_r_def;
-val r = translate aig_cert_encodeTheory.qinterv_live_r_l_def;
-val r = translate aig_cert_encodeTheory.qinterv_live_lr_r_def;
-val r = translate aig_cert_encodeTheory.qinterv_live_ll_r_def;
-val r = translate aig_cert_encodeTheory.qinterv_live_ll_lr_def;
+val r = translate xaig_cert_encodeTheory.encode_liveness_cond_def;
+val r = translate xaig_cert_encodeTheory.encode_decrease_cond_def;
+val r = translate xaig_cert_encodeTheory.encode_closure_cond_def;
+val r = translate xaig_cert_encodeTheory.encode_stable_cond_def;
 
-val r = translate aig_cert_encodeTheory.encode_signal_imply_aux_def;
-val r = translate aig_cert_encodeTheory.encode_signal_imply_def;
-
-val r = translate aig_cert_encodeTheory.encode_lives_hold_aux_def;
-val r = translate aig_cert_encodeTheory.encode_lives_hold_def;
-
-val r = translate aig_cert_encodeTheory.encode_reset_cond_def;
-val r = translate aig_cert_encodeTheory.encode_transition_cond_def;
-val r = translate aig_cert_encodeTheory.encode_safety_cond_def;
-val r = translate aig_cert_encodeTheory.encode_base_cond_def;
-val r = translate aig_cert_encodeTheory.encode_induction_cond_def;
-
-val r = translate aig_cert_encodeTheory.encode_liveness_cond_def;
-val r = translate aig_cert_encodeTheory.encode_decrease_cond_def;
-val r = translate aig_cert_encodeTheory.encode_closure_cond_def;
-val r = translate aig_cert_encodeTheory.encode_stable_cond_def;
-
-val r = translate aig_cert_encodeTheory.aig_lookup_def;
-val r = translate aig_cert_encodeTheory.latch_deps_def;
-val r = translate aig_cert_encodeTheory.reset_edges_def;
-val r = translate aig_cert_encodeTheory.reset_graph_def;
+val r = translate xaig_cert_encodeTheory.xaig_lookup_def;
+val r = translate xaig_cert_encodeTheory.latch_deps_def;
+val r = translate xaig_cert_encodeTheory.reset_edges_def;
+val r = translate xaig_cert_encodeTheory.reset_graph_def;
 
 val r = translate sptreeTheory.mk_BN_def;
 val r = translate sptreeTheory.mk_BS_def;
@@ -129,8 +124,6 @@ val r = translate topological_sortTheory.partition_def;
 val r = translate topological_sortTheory.top_sort_aux_def;
 val r = translate topological_sortTheory.top_sort_def;
 
-(* TODO potential inefficiency: unnecessary conversion to num.
-     It might be more efficient for latch_deps to be directly over sptree/num_set *)
 val r = translate topological_sortTheory.to_nums_def;
 val r = translate topological_sortTheory.top_sort_any_def;
 
@@ -144,4 +137,4 @@ val _ = top_sort_any_side |> update_precondition;
 val r = translate
           (topological_sortTheory.has_cycle_def |> REWRITE_RULE [MEMBER_INTRO]);
 
-val r = translate aig_cert_encodeTheory.stratified_cond_def;
+val r = translate xaig_cert_encodeTheory.stratified_cond_def;
