examples/hwmcc_checker/translation/aig_to_cnfProgScript.sml
@@ -1,121 +1,115 @@
 (*
-  Translates aig_to_cnf (and its dependencies on cnf).
+  Translates xaig_to_cnf (and its dependencies on xaig).
 *)
 Theory aig_to_cnfProg
 Ancestors
   ml_translator  (* MEMBER_INTRO *)
-  aig_fmapsProg aig_to_cnf
+  aig_fmapsProg xaig_to_cnf aig_to_cnf
 Libs
   preamble ml_translatorLib
 
 val _ = translation_extends "aig_fmapsProg";
 
+(* The xaig definitions name the gate, input and latch type variables
+   'a, 'i and 'l. *)
+fun xinst (a, b, c) =
+  INST_TYPE [alpha |-> a, mk_vartype "'i" |-> b, mk_vartype "'l" |-> c];
+
+val nnn = xinst (“:num”, “:num”, “:num”);
+
+(*----------------------------------------------------------------------*
+   the parsed circuit: xor/ite detection
+ *----------------------------------------------------------------------*)
+
+val r = translate (xaig_to_cnfTheory.match_xor_def |> nnn);
+val r = translate (xaig_to_cnfTheory.match_ite_def |> nnn);
+val r = translate (xaig_to_cnfTheory.optimize_gate_def |> nnn);
+val r = translate (xaig_to_cnfTheory.add_and_def |> nnn);
+val r = translate (xaig_to_cnfTheory.xaig_opt_rev_def |> nnn);
+
+(*----------------------------------------------------------------------*
+   the lowering to CNF
+
+   Renaming hands out num names, so everything from here on is monomorphic
+   whatever the encoded condition was named by.
+ *----------------------------------------------------------------------*)
+
 val r = translate cnfTheory.negate_def;
-val r = translate aig_to_cnfTheory.eq_every_to_cnf_def;
-val r = translate aig_to_cnfTheory.not_TT_def;
-val r = translate aig_to_cnfTheory.var_to_num_def;
-val r = translate aig_to_cnfTheory.var_to_lit_def;
-val r = translate (aig_to_cnfTheory.and_to_cnf_def |> REWRITE_RULE [MEMBER_INTRO]);
-val r = translate aig_to_cnfTheory.to_cnf_def;
-val r = translate aig_to_cnfTheory.direct_aig_to_cnf_def;
+
+val r = translate xaig_to_cnfTheory.xvar_to_num_def;
+val r = translate xaig_to_cnfTheory.xvar_to_lit_def;
+val r = translate xaig_to_cnfTheory.eq_every_pos_def;
+val r = translate xaig_to_cnfTheory.eq_every_neg_def;
+val r = translate xaig_to_cnfTheory.or_every_pos_def;
+val r = translate xaig_to_cnfTheory.or_every_neg_def;
+val r = translate xaig_to_cnfTheory.xor_pos_def;
+val r = translate xaig_to_cnfTheory.xor_neg_def;
+val r = translate xaig_to_cnfTheory.ite_pos_def;
+val r = translate xaig_to_cnfTheory.ite_neg_def;
+val r = translate xaig_to_cnfTheory.gty_pos_def;
+val r = translate xaig_to_cnfTheory.gty_neg_def;
+val r = translate xaig_to_cnfTheory.xgty_to_cnf_def;
+
+(* The polarity map is keyed by the renamed gate names; neither definition
+   mentions a literal, so nothing in them pins the key type down. *)
+val to_num = INST_TYPE [alpha |-> “:num”];
+
+val r = translate (xaig_to_cnfTheory.pol_of_def |> to_num);
+val r = translate xaig_to_cnfTheory.flip_pol_def;
+val r = translate (xaig_to_cnfTheory.add_pol_def |> to_num);
+val r = translate xaig_to_cnfTheory.add_lit_pol_def;
+val r = translate xaig_to_cnfTheory.gty_pols_def;
+val r = translate xaig_to_cnfTheory.add_lits_pol_def;
+val r = translate xaig_to_cnfTheory.add_gty_pol_def;
+val r = translate xaig_to_cnfTheory.xto_cnf_def;
+val r = translate xaig_to_cnfTheory.direct_xaig_to_cnf_def;
+
+(*----------------------------------------------------------------------*
+   pruning and renaming an encoded condition
+
+   One instance per gate name type of the nine conditions; reset and safety
+   share one, as do closure and stable.
+ *----------------------------------------------------------------------*)
 
 fun translate_rest i = let
+  val r = translate (xaig_to_cnfTheory.gty_lits_def |> i)
   val r = translate (aig_to_cnfTheory.new_live_def |> i)
-  val r = translate (aig_to_cnfTheory.prune_rev_def |> i)
-  val r = translate (aig_to_cnfTheory.prune_for_def |> i)
-  val r = translate (aig_to_cnfTheory.aig_rename_aux_def |> i)
-  val r = translate (aig_to_cnfTheory.aig_rename_rev_def |> i)
-  val r = translate (aig_to_cnfTheory.aig_to_cnf_def |> i)
+  val r = translate (xaig_to_cnfTheory.xprune_rev_def |> i)
+  val r = translate (xaig_to_cnfTheory.xprune_for_def |> i)
+  val r = translate (xaig_to_cnfTheory.xrename_lit_def |> i)
+  val r = translate (xaig_to_cnfTheory.xrename_lits_def |> i)
+  val r = translate (xaig_to_cnfTheory.xrename_gty_def |> i)
+  val r = translate (xaig_to_cnfTheory.xaig_rename_rev_def |> i)
+  val r = translate (xaig_to_cnfTheory.xaig_to_cnf_def |> i)
   in r end
 
-(* By instantiating the types, the translator should translate finite maps
-   with something more efficient than alists, assuming aig_fmapsProgScript.sml
-   contains the appropriate comparison functions.
+(* the parsed circuits *)
+val r = translate_rest nnn;
 
-   The general type for AIGs is ('α, 'β, 'γ) aig.
- *)
+(* reset, safety *)
+val r = translate_rest (xinst (“:(num + num) ext”, “:num”, “:num”));
 
-(* TODO Instead of big types, add type abbreviations and use them everywhere
-   (aig_cert_encode, aig_fmapsProg, here) *)
+(* transition *)
+val r = translate_rest
+  (xinst (“:((num + num) + (num + num)) ext”, “:num + num”, “:num + num”));
 
-(*
-  For encode_reset_cond
-*)
-val i = INST_TYPE
-          [alpha |-> “:(num + num) iext”,
-           beta  |-> “:num”,
-           gamma |-> “:num”]
-val r = translate_rest i;
+(* base *)
+val r = translate_rest (xinst (“:num ext”, “:num”, “:num”));
 
-(*
-  For encode_transition_cond
-*)
-val i = INST_TYPE
-          [alpha |-> “:((num + num) iext + (num + num) iext) iext”,
-           beta  |-> “:num + num”,
-           gamma |-> “:num + num”]
-val r = translate_rest i;
+(* induction *)
+val r = translate_rest
+  (xinst (“:(num + num) ext”, “:num + num”, “:num + num”));
 
-(*
-  For encode_safety_cond
-*)
-val i = INST_TYPE
-          [alpha |-> “:(num + num) iext”,
-           beta  |-> “:num”,
-           gamma |-> “:num”]
-val r = translate_rest i;
+(* liveness *)
+val r = translate_rest
+  (xinst (“:(((num + num) + (num + num)) + (num + num)) ext”,
+          “:num + num”, “:num + num”));
 
-(*
-  For encode_base_cond
-*)
-val i = INST_TYPE
-          [alpha |-> “:num iext”,
-           beta  |-> “:num”,
-           gamma |-> “:num”]
-val r = translate_rest i;
+(* decrease *)
+val r = translate_rest
+  (xinst (“:((num + num) + num) ext”, “:num + num”, “:num + num”));
 
-(*
-  For encode_induction_cond
-*)
-val i = INST_TYPE
-          [alpha |-> “:(num iext + num iext) iext”,
-           beta  |-> “:num + num”,
-           gamma |-> “:num + num”]
-val r = translate_rest i;
-
-(*
-  For encode_liveness_cond
-*)
-val i = INST_TYPE
-          [alpha |-> “:(((num + num) iext + (num + num) iext) iext + (num + num) iext) iext”,
-           beta  |-> “:num + num”,
-           gamma |-> “:num + num”]
-val r = translate_rest i;
-
-(*
-  For encode_decrease_cond
-*)
-val i = INST_TYPE
-          [alpha |-> “:((num iext + num iext) iext + num iext) iext”,
-           beta  |-> “:num + num”,
-           gamma |-> “:num + num”]
-val r = translate_rest i;
-
-(*
-  For encode_closure_cond
-*)
-val i = INST_TYPE
-          [alpha |-> “:((((num iext + num iext) iext + num iext) iext + num iext) iext + num iext) iext”,
-           beta  |-> “:(num + num) + num”,
-           gamma |-> “: (num + num) + num”]
-val r = translate_rest i;
-
-
-(*
-  For encode_stable_cond
-*)
-val i = INST_TYPE
-          [alpha |-> “:(((num iext + num iext) iext + num iext) iext + (num + num) iext) iext”,
-           beta  |-> “:(num + num) + num”,
-           gamma |-> “: (num + num) + num”]
-val r = translate_rest i;
+(* closure, stable *)
+val r = translate_rest
+  (xinst (“:(((num + num) + num) + (num + num)) ext”,
+          “:(num + num) + num”, “:(num + num) + num”));
