examples/hwmcc_checker/translation/README.md
@@ -1,22 +1,22 @@
 Translation scripts.
 
 [aigProgScript.sml](aigProgScript.sml):
-Translates aig.
+Translates aig and xaig.
 
 [aig_cert_encodeProgScript.sml](aig_cert_encodeProgScript.sml):
-Translates aig_cert_encode.
+Translates xaig_cert_encode.
 
 [aig_cert_fullProgScript.sml](aig_cert_fullProgScript.sml):
 Translates aig_cert_full.
 
 [aig_fmapsProgScript.sml](aig_fmapsProgScript.sml):
-Setting up translator for the fmap instances that are used in aig_to_cnf.
+Setting up translator for the fmap instances that are used in xaig_to_cnf.
 
 [aig_parseProgScript.sml](aig_parseProgScript.sml):
 Translates aig_parse.
 
 [aig_to_cnfProgScript.sml](aig_to_cnfProgScript.sml):
-Translates aig_to_cnf (and its dependencies on cnf).
+Translates xaig_to_cnf (and its dependencies on xaig).
 
 [cake_tigerProgProofScript.sml](cake_tigerProgProofScript.sml):
 Proofs for the top-level binary cake_tiger.
